theories/lang/cpp/logic/new_delete.v
@@ -137,7 +137,7 @@ Module Type Expr__newdelete.
                           [| new_args <> nil |] ** Q (Vptr storage_ptr) free
                         else
                           (* [blockR sz -|- tblockR aty] *)
-                          (storage_ptr |-> (blockR sz 1 ** alignedR al) **
+                          (storage_ptr |-> (blockR sz (CV.m 1) ** alignedR al) **
                            (* TODO: ^ This misses an condition that [storage_ptr]
                               is suitably aligned, accounting for
                               __STDCPP_DEFAULT_NEW_ALIGNMENT__ (issue #149) *)
@@ -147,21 +147,23 @@ Module Type Expr__newdelete.
                                   provides_storage storage_ptr obj_ptr aty -*
                                   match oinit with
                                   | None => (* default_initialize the memory *)
-                                    default_initialize aty obj_ptr
-                                                       (fun free' =>
-                                                          (* Track the type we are allocating
-                                                             so it can be checked at [delete]
-                                                           *)
-                                                          obj_ptr |-> new_tokenR 1 aty -*
-                                                          Q (Vptr obj_ptr) (free' >*> free))
+                                    default_initialize false aty obj_ptr
+                                      (fun free' =>
+                                         (* Track the type we are allocating
+                                            so it can be checked at [delete].
+                                            It is important that this preseves
+                                            `const`ness of the type.
+                                          *)
+                                         obj_ptr |-> new_tokenR 1 aty -*
+                                         Q (Vptr obj_ptr) (free' >*> free))
                                   | Some init => (* Use [init] to initialize the memory *)
                                     wp_initialize aty obj_ptr init
-                                            (fun free' =>
-                                               (* Track the type we are allocating
-                                                  so it can be checked at [delete]
-                                                *)
-                                               obj_ptr |-> new_tokenR 1 aty -*
-                                               Q (Vptr obj_ptr) (free' >*> free))
+                                      (fun free' =>
+                                         (* Track the type we are allocating
+                                            so it can be checked at [delete]
+                                          *)
+                                         obj_ptr |-> new_tokenR 1 aty -*
+                                         Q (Vptr obj_ptr) (free' >*> free))
                                   end))))))
         |-- wp_operand (Enew new_fn new_args aty None oinit) Q.
 
@@ -210,7 +212,7 @@ Module Type Expr__newdelete.
                             [| new_args <> nil |] ** Q (Vptr storage_ptr) free
                           else
                             (* [blockR sz -|- tblockR (Tarray aty array_size)] *)
-                            (storage_ptr |-> blockR (sz' + sz) 1 **
+                            (storage_ptr |-> blockR (sz' + sz) (CV.m 1) **
                              storage_ptr .[Tu8 ! sz'] |-> alignedR al) **
                              (* todo: ^ This misses an condition that [storage_ptr]
                               is suitably aligned, accounting for
@@ -223,7 +225,7 @@ Module Type Expr__newdelete.
                                      obj_ptr array_ty -*
                                    match oinit with
                                    | None => (* default_initialize the memory *)
-                                     default_initialize array_ty obj_ptr
+                                     default_initialize false array_ty obj_ptr
                                                         (fun free'' =>
                                                            (* Track the type we are allocating
                                                               so it can be checked at [delete]
@@ -324,6 +326,8 @@ Module Type Expr__newdelete.
           iApply resolve_virtual_frame. iIntros (???); iApply "X".
         Qed.
 
+        Definition cv_compat (t1 t2 : type) : Prop :=
+          erase_qualifiers t1 = erase_qualifiers t2.
 
         (* delete
 
@@ -364,7 +368,8 @@ Module Type Expr__newdelete.
              else
                (* v---- Calling destructor with object pointer *)
                resolve_dtor destroyed_type obj_ptr (fun this' mdc_ty =>
-                    this' |-> new_tokenR 1 mdc_ty **
+                    Exists cv_mdc, this' |-> new_tokenR 1 cv_mdc **
+                                   [| cv_compat cv_mdc mdc_ty |] **
                     (* v---- because dispatch could be virtual, the translation unit
                              used to destroy the object may need to be different *)
                     Exists tu', denoteModule tu' ** destroy_val tu' mdc_ty this' (
@@ -374,7 +379,7 @@ Module Type Expr__newdelete.
                       (* Transfer memory to underlying storage pointer; unlike in
                          [end_provides_storage], this memory was pre-destructed by
                          [delete_val]. *)
-                      (storage_ptr |-> blockR sz 1 -*
+                      (storage_ptr |-> blockR sz (CV.m 1) -*
                        (* v---- Calling deallocator with storage pointer
                                 Like above, because the operation is on the MDC,
                                 we must use [tu'] *)
@@ -414,7 +419,7 @@ Module Type Expr__newdelete.
                       (* Transfer memory to underlying storage pointer; unlike in
                          [end_provides_storage], this memory was pre-destructed by
                          [delete_val]. *)
-                      (storage_ptr |-> blockR (sz' + sz) 1 -*
+                      (storage_ptr |-> blockR (sz' + sz) (CV.m 1) -*
                        (* v---- Calling deallocator with storage pointer.
                           Note: we rely on the AST to have correctly resolved this since the dispatch is statically known.
                         *)
