theories/lang/cpp/logic/stmt.v
@@ -7,7 +7,8 @@ Require Import iris.proofmode.proofmode.
 
 From bedrock.lang.cpp Require Import ast semantics.
 From bedrock.lang.cpp.logic Require Import
-     pred path_pred heap_pred destroy wp initializers call.
+     pred path_pred heap_pred destroy
+     wp initializers.
 Require Import bedrock.lang.bi.errors.
 
 Module Type Stmt.
@@ -69,13 +70,12 @@ Module Type Stmt.
                (k : region -> FreeTemp -> epred)
       : mpred :=
       Forall (addr : ptr),
-        let rty := erase_qualifiers ty in
         let destroy frees :=
-            interp frees (k (Rbind x addr ρ) (FreeTemps.delete rty addr))
+            interp frees (k (Rbind x addr ρ) (FreeTemps.delete ty addr))
         in
         match init with
         | Some init => wp_initialize ρ_init ty addr init $ fun frees => destroy frees
-        | None => default_initialize ty addr (fun frees => destroy frees)
+        | None => default_initialize false ty addr (fun frees => destroy frees)
         end.
 
     Lemma wp_decl_var_frame : forall x ρ ρ_init init ty (k k' : region -> FreeTemps -> epred),
@@ -105,7 +105,7 @@ Module Type Stmt.
       | Dinit ts nm ty init =>
         let do_init :=
             match init with
-            | None => default_initialize ty (_global nm) (k ρ)
+            | None => default_initialize false ty (_global nm) (k ρ)
             | Some init => wp_initialize ρ_init ty (_global nm) init (k ρ)
             end
         in
